# Week 2 - Lab Sheet

Do as much as you can in the lab, and complete the remaining exercises in your own time. Feel free to ask questions on Teams in the channel `lab`. But don't give spoilers there.

```agda
module lab2 where

open import prelude hiding (if_then_else_;_||_)
private
```

## Part I: Booleans

### Section 1: Operations on Booleans

#### Exercise 1.1

We have already defined `if-then-else` like so:

```agda
 if_then_else_ : {A : Type} ‚Üí Bool ‚Üí A ‚Üí A ‚Üí A
 if true  then x else y = x
 if false then x else y = y
```

But this requires our two branches to be of the same type A. Instead, we could
define `if-then-else` to have branches of different types, using the `_‚àî_`
type constructor.

```agda
 if'_then_else_ : {A B : Type} ‚Üí Bool ‚Üí A ‚Üí B ‚Üí A ‚àî B
 if' true then x else y = inl x
 if' false then x else y = inr y
```

**Define** this function.

#### Exercise 1.2

We can define the `_||_` function in (at least) two different ways, depending on
how much pattern-matching we wish to perform:

```agda
 _||_ : Bool ‚Üí Bool ‚Üí Bool
 true  || y = true
 false || y = y

 _||'_ : Bool ‚Üí Bool ‚Üí Bool
 true  ||' true  = true
 true  ||' false = true
 false ||' true  = true
 false ||' false = false
```

**Complete** the two holes for `_||_` and the four holes for `_||'_`.

The `_||_` operator is *associative*, meaning `a || (b || c) ‚â° (a || b) || c`.

We can prove this for both of our definitions:

```agda
 ||-assoc : (a b c : Bool)  ‚Üí a ||  (b ||  c) ‚â° (a ||  b) || c
 ||-assoc true b c = refl (true || (b || c))
 ||-assoc false b c = refl ( false || (b || c))

 ||'-assoc : (a b c : Bool) ‚Üí a ||' (b ||' c) ‚â° (a ||' b) ||' c
 ||'-assoc true true true = refl (true ||' (true ||' true))
 ||'-assoc true true false = refl (true ||' (true ||' false))
 ||'-assoc true false true = refl (true ||' (false ||' true))
 ||'-assoc true false false = refl (true ||' (false ||' false))
 ||'-assoc false true true = refl (false ||' (true ||' true))
 ||'-assoc false true false = refl (false ||' (true ||' false))
 ||'-assoc false false true = refl (false ||' (false ||' true ))
 ||'-assoc false false false = refl (false ||' (false ||' false))
```

**Complete** both of these proofs.

**Hint**. Try to use `refl` to prove equalities, which can be used when Agda calculates that two things are equal (see the [identity type](../identity-type.lagda.md) handout for more details).

**Hint**. Because `_||_` was defined by pattern matching on the first argument, it
may be helpful to use the same strategy.

Which of these did you prefer proving, and why?

#### Exercise 1.3

**Complete** the proof that Boolean disjunction is commutative:

```agda
 ||-is-commutative : (a b : Bool) ‚Üí a || b ‚â° b || a
 ||-is-commutative true true = refl true 
 ||-is-commutative true false  = refl true
 ||-is-commutative false true  = refl true
 ||-is-commutative false false = refl false
```

#### Exercise 1.4

**Complete** the proof that `false` is the left unit element of `_||_`:

```agda
 false-left-unit-for-|| : (b : Bool) ‚Üí false || b ‚â° b
 false-left-unit-for-|| true = refl true
 false-left-unit-for-|| false = refl false
```

**Complete** the proof that `false` is the right unit element of `_||_`:

```agda
 false-right-unit-for-|| : (b : Bool) ‚Üí b || false ‚â° b
 false-right-unit-for-|| true = refl true
 false-right-unit-for-|| false = refl false
```

#### Exercise 1.5

Now prove the analogous properties for `_&&_`.

**Complete** the proof that Boolean conjunction is associative:

```agda
 &&-is-associative : (a b c : Bool) ‚Üí a && (b && c) ‚â° (a && b) && c
 &&-is-associative true b c = refl ( b && c)
 &&-is-associative false b c = refl false
```

**Complete** the proof that Boolean conjunction is commutative:

```agda
 &&-is-commutative : (a b : Bool) ‚Üí a && b ‚â° b && a
 &&-is-commutative true true = refl true
 &&-is-commutative true false = refl false
 &&-is-commutative false true = refl false
 &&-is-commutative false false = refl false
```

**Complete** the proof that that `true` is the left unit element of `_&&_`:

```agda
 true-left-unit-for-&& : (b : Bool) ‚Üí true && b ‚â° b
 true-left-unit-for-&& true = refl true
 true-left-unit-for-&& false = refl false
```

**Complete** the proof that that `true` is the right unit element of `_&&_`:

```agda
 true-right-unit-for-&& : (b : Bool) ‚Üí b && true ‚â° b
 true-right-unit-for-&& true = refl true
 true-right-unit-for-&& false = refl false
```

#### Exercise 1.6

An important algebraic property between two operators is *distributivity*. For
example, multiplication distributes over addition since `x * (y + z) = (x * y) +
(x * z)` for every `x, y, z ‚àà ‚Ñï`. The same is the case for the Boolean
conjunction and disjunction operators we have defined.

**Complete** the proof that Boolean conjunction distributes over Boolean
disjunction:

```agda
 &&-distributes-over-|| : (a b c : Bool) ‚Üí a && (b || c) ‚â° (a && b) || (a && c)
 &&-distributes-over-|| true b c = refl (b || c)
 &&-distributes-over-|| false b c = refl false
```

```agda
 ||-distributes-over-&& : (a b c : Bool) ‚Üí a || (b && c) ‚â° (a || b) && (a || c)
 ||-distributes-over-&& true b c = refl true
 ||-distributes-over-&& false b c = refl (b && c)
```

### Section 2: Identity type and `Bool`

With these exercises, you will practise with the identity type and `Bool`.

#### Exercise 2.1

Recall how we defined `_‚â£_` for [natural
numbers](../introduction.lagda.md#the-empty-type-and-the-unit-type). We could do
the same for the Booleans.

```agda

 _‚â£_ : Bool ‚Üí Bool ‚Üí Type
 true ‚â£ true = ùüô
 true ‚â£ false = ùüò
 false ‚â£ true = ùüò
 false ‚â£ false = ùüô
```

**Define** this function.

Tip: you can type `‚â£` as `\===`.

#### Exercise 2.2

We can also define a Boolean-valued equality function.

```agda
 _==_ : Bool ‚Üí Bool ‚Üí Bool
 true == true = true
 true == false = false
 false == true = false
 false == false = true
```

**Define** this function.

#### Exercise 2.3

Now we write a conversion function from `x ‚â° y` to `x ‚â£ y`, just like the
function `back` in
[introduction](../introduction.lagda.md#the-identity-type-former-__).

```agda
 ‚â°-to-‚â£ : (x y : Bool) ‚Üí x ‚â° y ‚Üí x ‚â£ y
 ‚â°-to-‚â£ true true (refl true ) = ‚ãÜ
 ‚â°-to-‚â£ false false (refl .false) = ‚ãÜ


```

**Complete** this function.

#### Exercise 2.4

The following helper function makes some functions nicer to read.

```agda
 is-true : Bool ‚Üí Type
 is-true b = b ‚â° true
```

Now we can consider another conversion function.

```agda
 ‚â£-to-== : (x y : Bool) ‚Üí x ‚â£ y ‚Üí is-true (x == y)
 ‚â£-to-== true true e = refl true
 ‚â£-to-== false false e = refl true
```

**Define** this function.

#### Exercise 2.5

And similarly, we have

```agda
 ==-to-‚â° : (x y : Bool) ‚Üí is-true (x == y) ‚Üí x ‚â° y
 ==-to-‚â° true true e = refl true
 ==-to-‚â° false false e = refl false
```

**Define** this function.

#### Exercise 2.6

Finally, we can use the above functions to define the three remaining
implications

.```agda
 ‚â°-to-== : (x y : Bool) ‚Üí x ‚â° y ‚Üí is-true (x == y)
 ‚â°-to-== x y e = ‚â£-to-== x y (‚â°-to-‚â£ x y e)

 ‚â£-to-‚â° : (x y : Bool) ‚Üí x ‚â£ y ‚Üí x ‚â° y
 ‚â£-to-‚â° true true e = refl true
 ‚â£-to-‚â° false false e = refl false

 ==-to-‚â£ : (x y : Bool) ‚Üí is-true (x == y) ‚Üí x ‚â£ y
 ==-to-‚â£ true true e = ‚ãÜ
 ==-to-‚â£ false false e = ‚ãÜ
```

**Complete** these functions.


## Part II: Homework

First, take a look at how we define

 * the type of [natural numbers](../natural-numbers-type.lagda.md) and
 * the [identity type](../identity-type.lagda.md).

### Section 1: Some functions on natural numbers

#### Exercise 1.1

**Complete** the proof of the fact that `(suc x) + y ‚â° suc (x + y)`

```agda
 +-suc-on-left : (x y : ‚Ñï) ‚Üí (suc x) + y ‚â° suc (x + y)
 +-suc-on-left zero zero = refl (suc 0)
 +-suc-on-left zero (suc y) = refl (suc (suc y))
 +-suc-on-left (suc x) zero = refl (suc (suc (x + zero)))
 +-suc-on-left (suc x) (suc y) = refl (suc (suc (x + suc y)))

 +-suc-on-left' : (x y : ‚Ñï) ‚Üí (suc x) + y ‚â° suc (x + y)
 +-suc-on-left' x y = refl (suc (x + y))

```

#### Exercise 1.2

We can define the `max` operation on natural numbers as follows:

```agda
 max : ‚Ñï ‚Üí ‚Ñï ‚Üí ‚Ñï
 max zero    n       = n
 max (suc m) zero    = suc m
 max (suc m) (suc n) = suc (max m n)

```

**Define** the function `min` analogously:

```agda
 min : ‚Ñï ‚Üí ‚Ñï ‚Üí ‚Ñï
 min zero n = zero
 min (suc m) zero = zero
 min (suc m) (suc n) = suc (min m n)
```

### Section 2: Natural numbers and proofs using induction

The function `+-0-on-right` expresses the fact that `0` is a right unit of the
operation `_+_`. Notice how we use an inductive hypothesis (the recursive call)
in the proof. (Spelling this out, `IH` tells us that `x + 0 ‚â° x`, so that `ap
suc IH` witnesses that `suc (x + 0) ‚â° suc x`.)

```agda
 +-0-on-right : (x : ‚Ñï) ‚Üí x + 0 ‚â° x
 +-0-on-right zero    = refl zero
 +-0-on-right (suc x) = ap suc IH
  where
   IH : x + 0 ‚â° x -- IH is short for induction hypothesis
   IH = +-0-on-right x
```

Using similar induction hypotheses, try to complete the following exercises.


#### Exercise 2.1

**Complete** the proof:

```agda
 +-suc-on-right' : (x y : ‚Ñï) ‚Üí x + suc y ‚â° suc (x + y)
 +-suc-on-right' zero y = refl (suc y)
 +-suc-on-right' (suc x) y = ap suc (+-suc-on-right' x y )

 +-suc-on-right : (x y : ‚Ñï) ‚Üí x + suc y ‚â° suc (x + y)
 +-suc-on-right zero y = refl (suc y)
 +-suc-on-right (suc x) y = ap suc IH
   where
     IH : x + suc y ‚â° suc (x + y)
     IH = +-suc-on-right x y

```

#### Exercise 2.2

In algebra, an operator `_*_` is called idempotent iff `x * x = x` for every
`x`. `max` is an example of an idempotent operator:

**Complete** the hole to prove that `max` is idempotent:

```agda
-- max-idempotent : (x : ‚Ñï) ‚Üí max x x ‚â° x
-- max-idempotent zero = refl zero
-- max-idempotent (suc x) = ap suc (max-idempotent x)

 max-idempotent : (x : ‚Ñï) ‚Üí max x x ‚â° x
 max-idempotent zero = refl zero
 max-idempotent (suc x) = ap suc IH
   where
     IH : max x x ‚â° x
     IH = max-idempotent x
```

#### Exercise 2.3

**Complete** the hole by constructing a proof of the fact that `max` is a
commutative operator:

```agda
-- max-commutative : (x y : ‚Ñï) ‚Üí max x y ‚â° max y x
-- max-commutative zero zero = refl zero 
-- max-commutative zero (suc y) = refl (suc y)
-- max-commutative (suc x) zero = refl (suc x)
-- max-commutative (suc x) (suc y) = ap suc (max-commutative x y)

 max-commutative : (x y : ‚Ñï) ‚Üí max x y ‚â° max y x
 max-commutative zero zero = refl zero
 max-commutative zero (suc y) = refl (suc y)
 max-commutative (suc x) zero = refl (suc x)
 max-commutative (suc x) (suc y) = ap suc IH
   where
     IH : max x y ‚â° max y x
     IH = max-commutative x y

```

#### Exercise 2.4

Now recall that we defined `min` in Exercise 1.2. Similarly, we can show that
`min` is idempotent and commutative too.

**Complete** the proof that `min` is idempotent:

```agda
-- min-idempotent : (x : ‚Ñï) ‚Üí min x x ‚â° x
-- min-idempotent zero = refl zero
-- min-idempotent (suc x) = ap suc (min-idempotent x)

 min-idempotent : (x : ‚Ñï) ‚Üí min x x ‚â° x
 min-idempotent zero = refl zero
 min-idempotent (suc x) = ap suc IH
  where
    IH : min x x ‚â° x
    IH = min-idempotent x

```

#### Exercise 2.5

**Complete** the proof that `min` is commutative:

```agda
--min-commutative : (x y : ‚Ñï) ‚Üí min x y ‚â° min y x
--min-commutative zero zero = refl zero
--min-commutative zero (suc y) = refl zero
--min-commutative (suc x) zero = refl zero
-- min-commutative (suc x) (suc y) = ap suc (min-commutative x y)

 min-commutative : (x y : ‚Ñï) ‚Üí min x y ‚â° min y x
 min-commutative zero zero = refl zero
 min-commutative zero (suc y) = refl zero
 min-commutative (suc x) zero = refl zero
 min-commutative (suc x) (suc y) = ap suc IH
   where
     IH : min x y ‚â° min y x
     IH = min-commutative x y

```


Lecture 2 Notes

```agda

 ‚Ñï-elim' : {A : ‚Ñï ‚Üí Type}
       ‚Üí A 0
       ‚Üí ((k : ‚Ñï) ‚Üí A k ‚Üí A (suc k))
       ‚Üí (n : ‚Ñï) ‚Üí A n

 ‚Ñï-elim' {A} a f = h
   where
     h : (n : ‚Ñï) ‚Üí A n
     h 0       = a
     h (suc n) = f n (h n)
-- this is a form of induction, elimination principles can also be know as induction as we are prooving something for all of x, something will hold so we can proove it can hold for zero and then one 

-- h (suc n) = {f} doing C-c C-r will refine on the f to give: we do it on f as it has type A (suc k)
-- h (suc n) = f {n }14 {h n }15 where i can fill the holes 14 and 15

 module lecture-binary-sums where
 open import general-notation
```

 recall this definiiton
 data _‚àî_ (A B : Type) : Type where
   inl : A ‚Üí A ‚àî B
   inr : B ‚Üí A ‚àî B

 for the elimiation we need to prove (a : A) ‚Üí P (inl a) and (b : B) ‚Üí (inr b)

```agda

 ‚àî-elim' : {A B : Type} (C : A ‚àî B ‚Üí Type)
        ‚Üí ((x : A) ‚Üí C (inl x))
        ‚Üí ((y : B) ‚Üí C (inr y))
        ‚Üí (z : A ‚àî B) ‚Üí C z
 ‚àî-elim' C f g (inl x) = f x
 ‚àî-elim' C f g (inr y) = g y

 ‚àî-nondep-elim' : {A B C : Type}
              ‚Üí (A ‚Üí C)
              ‚Üí (B ‚Üí C)
              ‚Üí (A ‚àî B ‚Üí C)

 ‚àî-nondep-elim' f g (inl a) = f a
 ‚àî-nondep-elim' f g (inr b) = g b

```
